Revert "Supplier ddb key (#87)"
This reverts commit 9c0830bab2f36115a57667f8eb506e3fb23eceb2.

DynamoDbEncryption/runtimes/java/src/main/smithy-generated/software/amazon/cryptography/dynamoDbEncryption/IDynamoDbItemBranchKeyIdSupplier.java
@@ -1,0 +1,11 @@
+// Copyright Amazon.com Inc. or its affiliates. All Rights Reserved.
+// SPDX-License-Identifier: Apache-2.0
+// Do not modify this file. This file is machine generated, and any changes to it will be overwritten.
+package software.amazon.cryptography.dynamoDbEncryption;
+
+import software.amazon.cryptography.dynamoDbEncryption.model.GetBranchKeyIdFromItemInput;
+import software.amazon.cryptography.dynamoDbEncryption.model.GetBranchKeyIdFromItemOutput;
+
+public interface IDynamoDbItemBranchKeyIdSupplier {
+  GetBranchKeyIdFromItemOutput GetBranchKeyIdFromItem(GetBranchKeyIdFromItemInput nativeValue);
+}
