DynamoDbEncryption/dafny/DynamoDbEncryption/src/DynamoDbEncryptionBranchKeyIdSupplier.dfy
@@ -2,7 +2,6 @@
 // SPDX-License-Identifier: Apache-2.0
 
 include "DynamoToStruct.dfy"
-include "Util.dfy"
 
 module DynamoDbEncryptionBranchKeyIdSupplier {
   import opened AwsCryptographyDynamoDbEncryptionTypes
@@ -10,38 +9,33 @@ module DynamoDbEncryptionBranchKeyIdSupplier {
   import DDB = ComAmazonawsDynamodbTypes
   import opened Seq
   import opened Wrappers
-  import opened StandardLibrary.UInt
   import DynamoToStruct
   import Base64
-  import DynamoDbEncryptionUtil
-
-  const MPL_EC_PARTITION_NAME: UTF8.ValidUTF8Bytes := UTF8.EncodeAscii("aws-crypto-partition-name")
-  const MPL_EC_SORT_NAME: UTF8.ValidUTF8Bytes := UTF8.EncodeAscii("aws-crypto-sort-name")
 
   class DynamoDbEncryptionBranchKeyIdSupplier
     extends MPL.IBranchKeyIdSupplier
   {
-    const ddbKeyBranchKeyIdSupplier: IDynamoDbKeyBranchKeyIdSupplier
+    const ddbItemBranchKeyIdSupplier: IDynamoDbItemBranchKeyIdSupplier
 
     predicate ValidState()
       ensures ValidState() ==> History in Modifies
     {
       && History in Modifies
-      && ddbKeyBranchKeyIdSupplier.ValidState()
-      && ddbKeyBranchKeyIdSupplier.Modifies <= Modifies
-      && History !in ddbKeyBranchKeyIdSupplier.Modifies
+      && ddbItemBranchKeyIdSupplier.ValidState()
+      && ddbItemBranchKeyIdSupplier.Modifies <= Modifies
+      && History !in ddbItemBranchKeyIdSupplier.Modifies
     }
 
     constructor(
-      ddbKeyBranchKeyIdSupplier: IDynamoDbKeyBranchKeyIdSupplier
+      ddbItemBranchKeyIdSupplier: IDynamoDbItemBranchKeyIdSupplier
     )
-      requires ddbKeyBranchKeyIdSupplier.ValidState()
-      ensures this.ddbKeyBranchKeyIdSupplier == ddbKeyBranchKeyIdSupplier
-      ensures ValidState() && fresh(this) && fresh(History) && fresh(Modifies - ddbKeyBranchKeyIdSupplier.Modifies)
+      requires ddbItemBranchKeyIdSupplier.ValidState()
+      ensures this.ddbItemBranchKeyIdSupplier == ddbItemBranchKeyIdSupplier
+      ensures ValidState() && fresh(this) && fresh(History) && fresh(Modifies - ddbItemBranchKeyIdSupplier.Modifies)
     {
-      this.ddbKeyBranchKeyIdSupplier := ddbKeyBranchKeyIdSupplier;
+      this.ddbItemBranchKeyIdSupplier := ddbItemBranchKeyIdSupplier;
       History := new MPL.IBranchKeyIdSupplierCallHistory();
-      Modifies := {History} + ddbKeyBranchKeyIdSupplier.Modifies;
+      Modifies := {History} + ddbItemBranchKeyIdSupplier.Modifies;
     }
 
     predicate GetBranchKeyIdEnsuresPublicly(input: MPL.GetBranchKeyIdInput, output: Result<MPL.GetBranchKeyIdOutput, MPL.Error>)
@@ -56,66 +50,57 @@ module DynamoDbEncryptionBranchKeyIdSupplier {
       ensures GetBranchKeyIdEnsuresPublicly(input, output)
       ensures unchanged(History)
     {
+      // Get encoded SIGN_ONLY DDB attributes from encryption context
       var context := input.encryptionContext;
+      var prefix := UTF8.EncodeAscii("aws-crypto-attr.");
+
       var attrMap: DDB.AttributeMap := map[];
 
-      // Add partition key to map
-      :- Need(MPL_EC_PARTITION_NAME in context.Keys,
-        MPL.AwsCryptographicMaterialProvidersException(
-          message := "Invalid encryption context: Missing partition name"));
-      var partitionName := context[MPL_EC_PARTITION_NAME];
-      var partitionValueKey := DynamoDbEncryptionUtil.DDBEC_EC_ATTR_PREFIX + partitionName;
-      :- Need(partitionValueKey in context.Keys,
-        MPL.AwsCryptographicMaterialProvidersException(
-          message := "Invalid encryption context: Missing partition value"));
-      attrMap :- AddAttributeToMap(partitionValueKey, context[partitionValueKey], attrMap);
+      var ddbAttrKeys := set k <- context.Keys | prefix < k :: k;
+      var s' := ddbAttrKeys;
+      while s' != {}
+        invariant s' <= ddbAttrKeys
+        decreases s'
+      {
+        var ddbAttrKey :| ddbAttrKey in s';
+        var encodedAttrValue := context[ddbAttrKey];
 
-      if MPL_EC_SORT_NAME in context.Keys {
-        var sortName := context[MPL_EC_SORT_NAME];
-        var sortValueKey := DynamoDbEncryptionUtil.DDBEC_EC_ATTR_PREFIX + sortName;
-        :- Need(sortValueKey in context.Keys,
-          MPL.AwsCryptographicMaterialProvidersException(
-            message := "Invalid encryption context: Missing sort value"));
-        attrMap :- AddAttributeToMap(sortValueKey, context[sortValueKey], attrMap);
+        // Obtain attribute name from EC kvPair key
+        var ddbAttrNameBytes := ddbAttrKey[|prefix|..];
+        var ddbAttrName :- UTF8.Decode(ddbAttrNameBytes)
+            .MapFailure(e => MPL.AwsCryptographicMaterialProvidersException(message:=e));
+        :- Need(DDB.IsValid_AttributeName(ddbAttrName),
+            MPL.AwsCryptographicMaterialProvidersException(
+              message := "Invalid serialization of DDB Attribute in encryption context."));
+
+        // Obtain attribute value from EC kvPair value
+        var utf8DecodedVal :- UTF8.Decode(encodedAttrValue)
+            .MapFailure(e => MPL.AwsCryptographicMaterialProvidersException(message:=e));
+        var base64DecodedVal :- Base64.Decode(utf8DecodedVal)
+            .MapFailure(e => MPL.AwsCryptographicMaterialProvidersException(message:=e));
+        :- Need(|base64DecodedVal| >= 2,
+            MPL.AwsCryptographicMaterialProvidersException(
+              message := "Invalid serialization of DDB Attribute in encryption context."));
+        var typeId := base64DecodedVal[..2];
+        var serializedValue := base64DecodedVal[2..];
+        var ddbAttrValue :- DynamoToStruct.BytesToAttr(serializedValue, typeId, false)
+            .MapFailure(e => MPL.AwsCryptographicMaterialProvidersException(message:=e));
+
+        // Add to our AttributeMap
+        attrMap := attrMap[ddbAttrName := ddbAttrValue.val];
+
+        // Pop 'ddbAttrKey' off the map, so that we may continue iterating
+        s' := set k' | k' in s' && k' != ddbAttrKey :: k';
       }
-        
+
       // Get branch key id from these DDB attributes
-      var branchKeyIdR := ddbKeyBranchKeyIdSupplier.GetBranchKeyIdFromDdbKey(
-            GetBranchKeyIdFromDdbKeyInput(ddbKey := attrMap)
+      var branchKeyIdR := ddbItemBranchKeyIdSupplier.GetBranchKeyIdFromItem(
+            GetBranchKeyIdFromItemInput(ddbItem := attrMap)
           );
       var branchKeyIdOut :- branchKeyIdR.MapFailure(ConvertToMplError);
 
       return Success(MPL.GetBranchKeyIdOutput(branchKeyId:=branchKeyIdOut.branchKeyId));
     }
-  }
-
-  function method AddAttributeToMap(ddbAttrKey: seq<uint8>, encodedAttrValue: seq<uint8>, attrMap: DDB.AttributeMap)
-      : (res: Result<DDB.AttributeMap, MPL.Error>) 
-    requires |ddbAttrKey| >= |DynamoDbEncryptionUtil.DDBEC_EC_ATTR_PREFIX|
-  {
-    // Obtain attribute name from EC kvPair key
-    var ddbAttrNameBytes := ddbAttrKey[|DynamoDbEncryptionUtil.DDBEC_EC_ATTR_PREFIX|..];
-    var ddbAttrName :- UTF8.Decode(ddbAttrNameBytes)
-        .MapFailure(e => MPL.AwsCryptographicMaterialProvidersException(message:=e));
-    :- Need(DDB.IsValid_AttributeName(ddbAttrName),
-        MPL.AwsCryptographicMaterialProvidersException(
-          message := "Invalid serialization of DDB Attribute in encryption context."));
-
-    // Obtain attribute value from EC kvPair value
-    var utf8DecodedVal :- UTF8.Decode(encodedAttrValue)
-        .MapFailure(e => MPL.AwsCryptographicMaterialProvidersException(message:=e));
-    var base64DecodedVal :- Base64.Decode(utf8DecodedVal)
-        .MapFailure(e => MPL.AwsCryptographicMaterialProvidersException(message:=e));
-    :- Need(|base64DecodedVal| >= 2,
-        MPL.AwsCryptographicMaterialProvidersException(
-          message := "Invalid serialization of DDB Attribute in encryption context."));
-    var typeId := base64DecodedVal[..2];
-    var serializedValue := base64DecodedVal[2..];
-    var ddbAttrValue :- DynamoToStruct.BytesToAttr(serializedValue, typeId, false)
-        .MapFailure(e => MPL.AwsCryptographicMaterialProvidersException(message:=e));
-
-    // Add to our AttributeMap
-    Success(attrMap[ddbAttrName := ddbAttrValue.val])
   }
   
   function method ConvertToMplError(err: Error)
