DynamoDbEncryption/dafny/DynamoDbEncryption/src/Util.dfy
@@ -12,9 +12,6 @@ module DynamoDbEncryptionUtil {
   const ReservedPrefix := "aws_dbe_"
   const BeaconPrefix := "aws_dbe_b_"
   const VersionPrefix := "aws_dbe_v_"
-  
-  const DDBEC_ATTR_PREFIX := "aws-crypto-attr."
-  const DDBEC_EC_ATTR_PREFIX: UTF8.ValidUTF8Bytes := UTF8.EncodeAscii(DDBEC_ATTR_PREFIX)
 
   // string to Error
   function method E(s : string) : Error {
